Lemma/Vector/Sigmoid/eq/Div1Add1ExpNeg.lean
@@ -1,0 +1,17 @@
+import sympy.Basic
+import sympy.vector.functions
+
+
+@[main]
+private lemma main
+  [Exp α]
+-- given
+  (x : List.Vector α n) :
+-- imply
+  x.sigmoid = 1 / (1 + exp (-x)) := by
+-- proof
+  unfold List.Vector.sigmoid
+  rfl
+
+
+-- created on 2026-07-05
